preservation/determinism

double_anno/coq/rules.v.d
@@ -1,0 +1,2 @@
+rules.vo rules.glob rules.v.beautified: rules.v
+rules.vio: rules.v
