double_anno/coq/typing_tlc.v.d
@@ -1,0 +1,2 @@
+typing_tlc.vo typing_tlc.glob typing_tlc.v.beautified: typing_tlc.v ./syntaxtlc.vo
+typing_tlc.vio: typing_tlc.v ./syntaxtlc.vio
